start writing rewriter

src/ListUtil.v
@@ -27,3 +27,131 @@ Module FromNil.
     Local Definition tx : nth_error (2::1::0::nil) 3 = None := eq_refl.
   End _test.
 End FromNil.
+
+Module Decompose.
+  Section WithElementType.
+    Context {A : Type}.
+
+    Fixpoint decompose_find' (f : nat -> A -> bool) i acc l {struct l} :
+      option (list A * A * list A) :=
+      match l with
+      | nil => None
+      | cons x l => if f i x
+                    then Some (acc, x, l)
+                    else decompose_find' f (S i) (x :: acc) l
+      end.
+
+    Definition decompose_find f l := decompose_find' f 0 nil l.
+
+    Definition found f l a (x : A) b :=
+      l = rev_append a (x :: b) /\ f (length a) x = true.
+
+    Local Create HintDb listutil discriminated.
+    Local Hint Rewrite rev_append_rev
+          app_length
+          PeanoNat.Nat.add_1_r
+          rev_app_distr
+          rev_involutive : listutil.
+    Local Hint Rewrite <- app_assoc : listutil.
+    Local Ltac crush :=
+      repeat match goal with
+             | H : (_ :: _) = (_ :: _) |- _ => inversion H; clear H
+             | H : (rev _ ++ _ :: nil) = (rev _ ++ _ :: nil) |- _ =>
+               change (rev ?a ++ ?x :: nil) with (rev (x :: a)) in H;
+               eapply (f_equal (@rev _)) in H;
+               repeat rewrite rev_involutive in H
+             | H : (rev _) = (rev _) |- _ =>
+               eapply (f_equal (@rev _)) in H;
+               repeat rewrite rev_involutive in H
+             | _ => autorewrite with listutil in *;
+                    cbn [rev_append rev length app] in *;
+                    subst;
+                    intuition idtac
+             end.
+
+    Lemma found_inv f y l a x b :
+      found f (y :: l) a x b ->
+      (a = nil /\ (f 0 y = true)) \/
+      (exists a', a = (a' ++ y :: nil) /\
+                  found (fun i => f (S i)) l a' x b).
+    Proof.
+      cbv [found].
+      pattern a; eapply rev_ind.
+      - crush.
+      - right; eexists; crush.
+    Qed.
+
+    Lemma found_end_inv f y l a x b :
+      found f (rev (y :: l)) a x b ->
+      (b = nil /\ (f (length l) y = true)) \/
+      (exists b', b = (b' ++ y :: nil) /\
+                  found f (rev l) a x b').
+    Proof.
+      cbv [found].
+      pattern b; eapply rev_ind.
+      - crush.
+      - intros z b' _ [H H'].
+        replace (rev_append a (x :: b' ++ z :: nil)) with
+            (rev (z :: rev b' ++ x :: a)) in H by crush.
+        right; eexists; crush.
+    Qed.
+
+    Lemma decompose_find_spec f l :
+      match decompose_find f l with
+      | Some (a, x, b) => found f l a x b /\
+                          ~ exists c y d, found f (rev a) c y d
+      | None => ~ exists a x b, found f l a x b
+      end.
+    Proof.
+      enough (forall acc,
+                 (~ exists a x b, found f (rev acc) a x b) ->
+                 match decompose_find' f (length acc) acc l with
+                 | Some (a, x, b) =>
+                   found f (rev_append acc l) a x b /\
+                   ~ exists c y d, found f (rev a) c y d
+                 | None => ~ exists a x b, found f (rev_append acc l) a x b
+                 end) as H.
+      {
+        cbv [decompose_find].
+        specialize (H nil); cbn [rev length] in H.
+        refine ((fun H' => ltac:(clear H)) (H _)).
+        - destruct (decompose_find' f 0 nil l) as [[[??]?]|];
+            rewrite ?app_nil_r in H'; cbn [rev_append] in H'; intuition.
+        - intros (?&?&?&Hnil).
+          cbv [found rev] in Hnil.
+          rewrite rev_append_rev in Hnil.
+          eapply app_cons_not_nil; intuition eauto.
+      }
+      induction l as [|y l];
+        intros acc Hacc; cbn [decompose_find' rev_append app].
+      - rewrite rev_append_rev, app_nil_r; eauto.
+      - cbv [found].
+        remember (f (length acc) y) as b; destruct b;
+          try solve [intuition eauto].
+        eapply (IHl (y :: acc)).
+        intros (?&?&?&Hyacc).
+        eapply found_end_inv in Hyacc.
+        destruct Hyacc as [|[? ?]].
+        + intuition congruence.
+        + eapply Hacc; do 3 eexists; intuition eauto.
+    Qed.
+
+    Definition decompose_at l n : option (list A * list A) :=
+      match decompose_find (fun i _ => Nat.eqb i n) l with
+      | Some (a, x, b) => Some (a, x :: b)
+      | None => None
+      end.
+
+    Lemma decompose_at_correct l n : match decompose_at l n with
+                                     | Some (a, b) => l = rev_append a b
+                                     | None => True
+                                     end.
+    Proof.
+      cbv [decompose_at].
+      pose proof (decompose_find_spec (fun i _ => Nat.eqb i n) l) as H.
+      destruct (decompose_find _ _) as [[[??]?]|];
+        cbv [found] in H;
+        intuition idtac.
+    Qed.
+  End WithElementType.
+End Decompose.
